In preparation for the design of a "linking" extension, generalize the type of the extension core projection to
  forall i:nat, option (CoreSemantics G (cT i) M D)

where cT is a family of nat-indexed core types.  (Previously, extensions supported 
different core semantics at each index i, but all such semantics shared the 
same core type.)

veric/fs_extension.v
@@ -166,7 +166,7 @@ Definition get_fs := match s with mkxT _ _ fs => fs end.
 
 End selectors.
 
-Definition proj_core (s: xT) (i: nat) := if eq_nat_dec i 1 then Some (get_core s) else None.
+Definition proj_core (i: nat) (s: xT) := if eq_nat_dec i 1 then Some (get_core s) else None.
 Definition active := fun _: xT => 1.
 Definition runnable := fun (ge: genv) (s: xT) => 
   match at_external csem (get_core s), safely_halted csem ge (get_core s) with 
